Add paritioning function - Thank you Probie for the help

Tablaux/TableauxCalculi.v
@@ -1,10 +1,224 @@
 (* Imports *)
-Require Import List.
+Require Import Bool List String Datatypes.
 
-Inductive Result : Set :=
-  | closed : Result
-  | open : Result
+(*
+Definition PropVars : string.
+Axiom Varseq_dec : forall x y : PropVars, {x = y} + {x <> y}.
+*)
+
+Inductive PropF : Type :=
+ | Var : string -> PropF
+ | Bot : PropF
+ | Conj : PropF -> PropF -> PropF
+ | Disj : PropF -> PropF -> PropF
+ | Impl : PropF -> PropF -> PropF
 .
 
-Definition notClosedisOpen := (forall A : Result, A <> closed -> A = open).
+Notation "# P" := (Var P) (at level 1).
+Notation "A ∨ B" := (Disj A B) (at level 15, right associativity).
+Notation "A ∧ B" := (Conj A B) (at level 15, right associativity).
+Notation "A → B" := (Impl A B) (at level 16, right associativity).
+Notation "⊥" := Bot (at level 0).
+Definition Neg A := A → ⊥.
+Notation "¬ A" := (Neg A) (at level 5).
+Definition Top := ¬⊥.
+Notation "⊤" := Top (at level 0).
+Definition BiImpl A B := (A→B)∧(B→A).
+Notation "A ↔ B" := (BiImpl A B) (at level 17, right associativity).
 
+(* Defining equivalence for PropF *)
+Fixpoint EquivPropF x y :=
+  match (x, y) with
+  | (# a, #b) => if string_dec a b then true else false
+  | (⊥, ⊥) => true
+  | (a1 ∧ a2, b1 ∧ b2) => andb (EquivPropF a1 b1) (EquivPropF a2 b2)
+  | (a1 ∨ a2, b1 ∨ b2) => andb (EquivPropF a1 b1) (EquivPropF a2 b2)
+  | (a1 → a2, b1 → b2) => andb (EquivPropF a1 b1) (EquivPropF a2 b2)
+  | (_, _) => false
+  end.
+
+(* Basic set of PropF *)
+Definition PropFSet : Type := list PropF.
+
+(* Possible Results after proof search *)
+Inductive Results :=
+  | Open
+  | Closed
+  | Failure
+.
+
+(* Defining a tableau rule *)
+Definition Numerator := PropFSet.
+Definition Denominator := sum (list PropFSet) Results.
+
+Definition Rule := prod Numerator Denominator.
+
+Definition getNumerator (rule : Rule) := fst rule.
+Definition getDenominator (rule : Rule) := snd rule.
+
+(* Method to get propsitional variables *)
+Fixpoint getPropVar (prop : PropF) :=
+  match prop with
+  | # pv => pv::nil
+  | ⊥ => nil
+  | a ∧ b => getPropVar a ++ getPropVar b
+  | a ∨ b => getPropVar a ++ getPropVar b
+  | a → b => getPropVar a ++ getPropVar b
+  end.
+
+Fixpoint getPropVars (props : PropFSet) :=
+  match props with
+  | nil => nil
+  | x::xs => getPropVar x ++ getPropVars xs
+  end.
+
+Fixpoint isInstanceOf (formula : PropF) (scheme : PropF) :=
+  match (formula, scheme) with
+  | (_, #b) => true
+  | (⊥, ⊥) => true
+  | (a1 ∧ a2, b1 ∧ b2) => andb (isInstanceOf a1 b1) (isInstanceOf a2 b2)
+  | (a1 ∨ a2, b1 ∨ b2) => andb (isInstanceOf a1 b1) (isInstanceOf a2 b2)
+  | (a1 → a2, b1 → b2) => andb (isInstanceOf a1 b1) (isInstanceOf a2 b2)
+  | (_, _) => false
+  end.
+
+Definition partitionTuple := list (PropF * PropF).
+
+(* Fix with fail monad or something ... *)
+Fixpoint matchVarHelp (scheme : PropF) (γ : PropF) : partitionTuple :=
+  match (scheme, γ) with
+  | (# pv, x) => (# pv, x)::nil
+  | (⊥, ⊥) => nil
+  | (a1 ∧ a2, b1 ∧ b2) => matchVarHelp a1 b1 ++ matchVarHelp a2 b2
+  | (a1 ∨ a2, b1 ∨ b2) => matchVarHelp a1 b1 ++ matchVarHelp a2 b2
+  | (a1 → a2, b1 → b2) => matchVarHelp a1 b1 ++ matchVarHelp a2 b2
+  | (_, _) => nil
+  end.
+
+Definition matchVar (scheme : PropF) (γ : PropF) :=
+  if isInstanceOf γ scheme then Some (matchVarHelp scheme γ)
+  else None.
+
+Recursive Extraction matchVar.
+
+Compute (matchVar (# "p" → # "r") (⊥ → (# "q"))).
+
+Fixpoint getSetVars (π : partitionTuple) : PropFSet :=
+  match π with
+  | nil => nil
+  | x::xs => (snd x) :: getSetVars xs
+  end.
+
+Compute getSetVars ((# "p", ⊥) :: (# "r", # "q") :: nil).
+
+Fixpoint lookupPartition (γ : PropF) (π : partitionTuple) :=
+  match π with
+  | nil => None
+  | (v1, v2)::xs => if EquivPropF γ v1 then Some v2
+                else lookupPartition γ xs
+  end.
+
+Fixpoint applyPartitionPropF (γ : PropF) (π : partitionTuple) :=
+  match lookupPartition γ π with
+  | None => 
+    match γ with
+    | # pv => # pv
+    | ⊥ => ⊥
+    | a1 ∧ a2 => applyPartitionPropF a1 π ∧ applyPartitionPropF a2 π
+    | a1 ∨ a2 => applyPartitionPropF a1 π ∨ applyPartitionPropF a2 π
+    | a1 → a2 => applyPartitionPropF a1 π → applyPartitionPropF a2 π
+    end
+  | Some x => x
+  end.
+
+Fixpoint applyPartition (Γ : PropFSet) (π : partitionTuple) :=
+  match Γ with
+  | nil => nil
+  | x::xs => (applyPartitionPropF x π) :: (applyPartition xs π)
+  end.
+
+Compute (applyPartition ((# "p" → # "r")::nil) ((# "p", ⊥) :: (# "r", # "q") :: nil)).
+
+Definition option_bind (A : Type) (B : Type) (x : option A) (f : A -> option B) :=
+  match x with
+  | None => None
+  | Some v => f v
+  end.
+
+Definition flip (A : Type) (B : Type) (C : Type) 
+  (f : B -> A -> C) (a : A) (b : B) := f b a.
+
+Fixpoint option_fold (A : Type) (B : Type)
+  (f : B -> A -> option B) (z : B) (l : list A) : option B :=
+    match l with
+    | nil => Some z
+    | x::xs => option_bind B B (option_fold A B f z xs) (flip A B (option B) f x)
+    end.
+
+Fixpoint inPartitionTuple p (π : partitionTuple) :=
+  match π with
+  | nil => false
+  | x::xs => if andb (EquivPropF (fst x) (fst p)) (EquivPropF (snd x) (snd p))
+              then true else inPartitionTuple p xs
+  end.
+
+Fixpoint usedVar (γ : PropF) (π : partitionTuple) :=
+  match π with
+  | nil => false
+  | x::xs => if (EquivPropF γ (fst x)) then true else usedVar γ xs
+  end.
+
+Fixpoint extendPartition (π1 π2 : partitionTuple) :=
+  match π2 with
+  | nil => Some π1
+  | x::xs => if inPartitionTuple x π1 then extendPartition π1 xs
+              else (if usedVar (fst x) π1 then None else extendPartition (x::π1) xs)
+  end.
+
+Check matchVar.
+
+Fixpoint partition_help (scheme : PropF) (Γ : PropFSet) (π : partitionTuple) :=
+  match Γ with
+  | nil => nil
+  | γ::γs =>
+    match matchVar scheme γ with
+    | None => partition_help scheme γs π
+    | Some π' =>
+      match extendPartition π π' with
+      | None => partition_help scheme γs π
+      | Some newπ => newπ :: partition_help scheme γs π
+      end
+    end
+  end.
+
+Check flat_map.
+
+Require Import Omega.
+Require Import Coq.Arith.Compare_dec.
+
+Lemma length_wf : forall A, well_founded (fun (xs : list A) ys => length xs < length ys).
+intros. unfold well_founded. induction a.
+constructor. intros. simpl in H. omega. constructor.
+intros. destruct (eq_nat_dec (length y) (length a0)).
+constructor. intros. apply IHa. rewrite <- e. exact H0.
+apply IHa. simpl in H. omega.
+Defined.
+
+Lemma unchanging : forall x π, length (applyPartition x π) <= length x.
+admit.
+Admitted.
+ 
+
+Definition partitions_help (schema : PropFSet) : PropFSet -> partitionTuple -> list partitionTuple.
+  refine (Fix (length_wf PropF) (fun _ => PropFSet -> partitionTuple -> list partitionTuple)
+   (fun schema f => (match schema as schema' return (schema = schema' -> PropFSet -> partitionTuple -> list partitionTuple) with
+    | nil => fun _ _ accπ => accπ::nil
+    | s::ss => fun H Γ accπ => let Π := partition_help s Γ accπ in
+        flat_map (fun π => f (applyPartition ss π) _ Γ π) Π
+    end) eq_refl) schema).
+    rewrite H. assert (length (applyPartition ss π) <= length ss) by apply unchanging.
+    simpl. omega.
+    Defined.
+
+
+Compute (partitions_help ((# "p" → # "q")::nil) ((⊥ → ⊥::# "r" → ⊥::nil)) nil).
