Tablaux/a_base.v
@@ -1,0 +1,37 @@
+Require Export List Bool.
+Set Implicit Arguments.
+
+Module Type base_mod.
+
+(* Defines the logical symbols *)
+
+Delimit Scope My_scope with M.
+Open Scope My_scope.
+
+Parameter PropVars : Set.
+Axiom Varseq_dec : forall x y:PropVars, {x = y} + {x <> y}.
+
+Inductive PropF : Set :=
+ | Var : PropVars -> PropF
+ | Bot : PropF
+ | Conj : PropF -> PropF -> PropF
+ | Disj : PropF -> PropF -> PropF
+ | Impl : PropF -> PropF -> PropF
+.
+
+Notation "# P" := (Var P) (at level 1) : My_scope.
+Notation "A ∨ B" := (Disj A B) (at level 15, right associativity) : My_scope.
+Notation "A ∧ B" := (Conj A B) (at level 15, right associativity) : My_scope.
+Notation "A → B" := (Impl A B) (at level 16, right associativity) : My_scope.
+Notation "⊥" := Bot (at level 0)  : My_scope.
+Definition Neg A := A → ⊥.
+Notation "¬ A" := (Neg A) (at level 5) : My_scope.
+Definition Top := ¬⊥.
+Notation "⊤" := Top (at level 0) : My_scope.
+Definition BiImpl A B := (A→B)∧(B→A).
+Notation "A ↔ B" := (BiImpl A B) (at level 17, right associativity) : My_scope.
+
+(* Test extraction *)
+Definition isBot x := if Varseq_dec x ⊥ then true else false.
+
+End base_mod.
