Tablaux/b_tableau.v
@@ -1,0 +1,7 @@
+Require Export a_base.
+Set Implicit Arguments.
+
+Module Type tableau_mod (X : base_mod).
+Import X.
+
+(* Includes tableau definition and the tableau rule definitions *)
